global/local path liveness reflection

lemma/liveness.v
@@ -473,12 +473,6 @@ Proof.
     }
 Qed.
 
-Lemma paired_assoc_head : forall t g l xs, 
-paired_path_assoc_cond (cocons (t,g,l) xs) -> assoc t g.
-Proof.
-    intros.
-    pinversion H;try apply always_mon;subst. simpl in H2;easy.
-Qed.
 
 Variant coseq_bisimI {A:Type} (R: coseq A -> coseq A -> Prop): 
 coseq A -> coseq A -> Prop :=
@@ -496,8 +490,258 @@ Variant path_assoc (R:local_path -> global_path -> Prop): local_path -> global_p
     R xs ys ->
    path_assoc R (cocons (gamma, l) xs) (cocons (g, l) ys)
    .
+
+Lemma path_assoc_mon : monotone2 path_assoc.
+Proof. red;intros. inversion IN;subst;constructor;try tauto. apply LE;easy. Qed.
    
 Definition path_assocC := paco2 path_assoc bot2.
+
+Definition conj_props (P:tctx -> Prop) (Q: gtt -> Prop) := forall gamma g,
+
+assoc gamma g -> (P gamma <-> Q g).
+
+Definition tctxREN_comm p q g := exists n, (tctxRE (lcomm p q n) g). 
+
+
+Definition tctxREN_send p q g := exists n s, (tctxRE (lsend p q s n) g).
+
+Definition tctxREN_recv p q g := exists n s, (tctxRE (lrecv p q s n) g).
+
+Print alwaysG.
+
+Definition wfg_global_path := alwaysCG (to_path_prop (fun a=> wfgC a /\ projectableA a) True).
+Definition wf_local_path := alwaysCG (to_path_prop tctx_wf True).
+Lemma global_path_always_wf : forall g l xs, wfgC g -> projectableA g -> global_valid_pathC (cocons (g,l) xs) -> 
+wfg_global_path (cocons (g,l) xs).
+Proof.
+    pcofix CIH.
+    intros * Hwfg Hprojable Hvalid.
+    pfold. constructor. simpl;easy.
+    destruct xs. left. pfold. constructor. easy.
+    right. destruct p.  pinversion Hvalid;subst;try apply valid_path_mon;try easy.
+    eapply CIH;
+    
+    red in H5; destruct l0;try tauto.
+    inversion Hvalid;subst.
+    eapply wfgC_after_step;try exact H5;try easy. eapply projectable_after_step;try exact H5;try easy.
+Qed.
+
+
+Lemma local_path_always_wf : forall g l xs, tctx_wf g -> local_valid_pathC (cocons (g,l) xs) -> 
+wf_local_path (cocons (g,l) xs).
+Proof.
+    pcofix CIH.
+    intros * Hwfg  Hvalid.
+    pfold. constructor. simpl;easy.
+    destruct xs. left. pfold. constructor. easy.
+    right. destruct p.  pinversion Hvalid;subst;try apply valid_path_mon;try easy.
+    eapply CIH;
+    
+    red in H5; destruct l0;try tauto.
+    inversion Hvalid;subst.
+    eapply tctx_wf_after_red_comm;try exact H5;try easy.
+Qed.
+
+
+Lemma path_assoc_eventually_enabled : forall xs ys P Q, wfg_global_path ys -> wf_local_path xs -> path_assocC xs ys -> 
+conj_props P Q -> eventually (to_path_prop  P False) xs -> eventually (to_path_prop  Q False) ys.
+Proof.
+    intros * Hwfgp Hwfgl Hpassoc Hconj Hevp.
+    generalize dependent ys.
+    induction Hevp.
+    {
+        intros. constructor. red in H. destruct xs;try easy.
+        pinversion Hpassoc;try apply path_assoc_mon;subst.
+        red.
+        eapply Hconj with (gamma:=gamma); easy. 
+    }
+    {
+     intros.
+     pinversion Hpassoc;try apply path_assoc_mon;subst.
+     constructor 2.
+     eapply IHHevp.
+     pinversion Hwfgl;try apply always_mon;subst;easy.
+     pinversion Hwfgp;try apply always_mon;subst;easy.
+     easy.   
+    }
+Qed.
+Lemma path_assoc_preserves_fairness_helper : forall xs p q ys, path_assocC xs ys ->
+eventually (headComm p q) xs -> eventually (headComm_global p q) ys.
+Proof.
+    intros * Hpassoc Hevp.
+    generalize dependent ys. induction Hevp.
+    {
+        intros. red in H. destruct xs as [ | [t l]];try easy.
+        destruct l;try tauto;destruct l;try tauto.
+        destruct (Nat.eq_dec p n);destruct (Nat.eq_dec q n0);try tauto;subst;clear H.
+        pinversion Hpassoc;try apply path_assoc_mon;subst. constructor. simpl. 
+        destruct (Nat.eq_dec n n);destruct (Nat.eq_dec n0 n0);tauto.    
+    }
+    {
+        intros * Hpassoc. pinversion Hpassoc;try apply path_assoc_mon;subst.
+        constructor 2.
+        eapply IHHevp. easy.  
+    }
+Qed.
+
+
+Lemma global_comm_enabled_assoc_local_comm_enabled: forall p q n gamma g, wfgC g ->
+tctx_wf gamma -> global_comm_enabled p q n g -> 
+assoc gamma g -> exists n', tctxRE (lcomm p q n') gamma.
+Proof.
+    intros * Hwfg Hwft Hgce Hassoc. 
+    red in Hgce. destr_hyps. eapply assoc_soundness with (gamma:=gamma) in H;try easy.
+    destr_hyps. exists x2. red. exists x0;easy.
+    pinversion H;subst;try apply step_mon;easy.
+Qed.
+
+Lemma wfg_global_path_head: forall g l ys, wfg_global_path (cocons (g,l) ys) -> wfgC g.
+Proof.
+    intros. pinversion H;try apply always_mon;subst. red in H2. tauto.
+Qed.
+
+Lemma wf_local_path_head: forall g l ys, wf_local_path (cocons (g,l) ys) -> tctx_wf g.
+Proof.
+    intros. pinversion H;try apply always_mon;subst. red in H2. tauto.
+Qed.
+
+Lemma always_tail {A:Type}: forall (g:A) (l:option label) xs P, alwaysCG P (cocons (g,l) xs) -> alwaysCG P xs.
+Proof. intros. pinversion H;try apply always_mon;subst. easy. Qed.
+
+
+    
+Lemma path_assoc_preserves_fairness : forall lp gp, wfg_global_path gp -> wf_local_path lp ->
+path_assocC lp gp ->
+fair_path lp -> fair_path_global gp.
+Proof.
+    pcofix CIH.
+    intros * Hwfgp Hwflp Hpassoc Hfairl.
+    pfold.
+    pinversion Hpassoc;try apply path_assoc_mon;subst.
+    {
+        constructor. red. intros. simpl in H. easy.
+    }
+    constructor.
+    { 
+        red. intros.
+        pinversion Hfairl;subst;try apply always_mon.
+        red in H4.
+        simpl in H1.
+        
+        eapply global_comm_enabled_assoc_local_comm_enabled in H1 as Hlc;try exact Hassoc;try easy;
+        try solve [
+        apply wfg_global_path_head in Hwfgp;easy | apply wf_local_path_head in Hwflp;easy].
+        destruct Hlc as [n' Hr].
+        
+        specialize (H4 p q n').
+        simpl in H4. 
+        specialize (H4 Hr). inversion H4;subst.
+        {  
+            simpl in H2.
+            destruct l;try tauto.
+            destruct l; destruct (Nat.eq_dec p n0);destruct (Nat.eq_dec q n1);subst;try tauto.
+            constructor 1. simpl. destruct (Nat.eq_dec n0 n0);
+            destruct (Nat.eq_dec n1 n1);tauto.     
+        }
+        {
+            constructor 2. eapply path_assoc_preserves_fairness_helper;try exact H3;try easy.
+        }   
+    }
+    {
+        right. eapply CIH with (lp := xs);
+        eapply always_tail in Hwfgp, Hwflp, Hfairl;try easy.
+    }
+Qed.
+
+Lemma local_send_enabled_global_send_enabled : forall g p q s n gamma, wfgC g -> tctx_wf gamma ->
+        assoc gamma g -> tctxRE (lsend p q (Some s) n) gamma ->
+        exists s' n', global_label_enabled (lsend p q (Some s') n') g.
+Proof.
+    intros * Hwfg Hwf Hassoc Hre.
+    destruct Hre as [t' Hre].
+    eapply lem_6_11a_tctx_send_invert in Hre. destr_hyps. 
+    
+    eapply assoc_inv_find in H as Hinvf;try exact Hassoc;try easy.
+    red in Hinvf. destr_hyps. eapply subtype_send_inv1 in H3 as Hst. destr_hyps;subst. 
+    eapply subtype_send_inv in H3. eapply Forall2R_prop in H3;try exact H0;tac_sanitize.
+    exists x4, n.
+    red. exists x2, x6. tauto.
+Qed.
+
+Lemma local_recv_enabled_global_recv_enabled : forall g p q s n gamma, wfgC g -> tctx_wf gamma ->
+    assoc gamma g -> tctxRE (lrecv p q (Some s) n) gamma ->
+    exists s' n', global_label_enabled (lrecv p q (Some s') n') g.
+Proof.
+    intros * Hwfg Hwf Hassoc Hre.
+    destruct Hre as [t' Hre].
+    eapply lem_6_11b_tctx_recv_invert in Hre. destr_hyps. 
+    
+    eapply assoc_inv_find in H as Hinvf;try exact Hassoc;try easy.
+    red in Hinvf. destr_hyps. eapply subtype_recv_inv1 in H3 as Hst. destr_hyps;subst.
+    
+    eapply projection_implies_wf in H2 as Hwfp;try easy.
+    eapply wfltt_slist_recv in Hwfp as Hslist. eapply slist_implies_some in Hslist.
+    destr_hyps. destruct x3. exists s0,x1.
+    red. exists x2, l. tauto.
+Qed.
+
+Lemma path_assoc_reflects_liveness_helper : forall xs p q ys, path_assocC xs ys ->
+eventually (headComm_global p q) ys -> eventually (headComm p q) xs.
+Proof.
+    intros * Hpassoc Hevp.
+    generalize dependent xs. induction Hevp.
+    {
+        intros. red in H. destruct xs as [ | [t l]];try easy.
+        destruct l;try tauto;destruct l;try tauto.
+        destruct (Nat.eq_dec p n);destruct (Nat.eq_dec q n0);try tauto;subst;clear H.
+        pinversion Hpassoc;try apply path_assoc_mon;subst. constructor. simpl. 
+        destruct (Nat.eq_dec n n);destruct (Nat.eq_dec n0 n0);tauto.    
+    }
+    {
+        intros * Hpassoc. pinversion Hpassoc;try apply path_assoc_mon;subst.
+        constructor 2.
+        eapply IHHevp. easy.  
+    }
+Qed.
+
+Lemma path_assoc_reflects_liveness : forall lp gp, wfg_global_path gp -> wf_local_path lp ->
+path_assocC lp gp ->
+live_path_global gp -> live_path lp.
+Proof.
+    pcofix CIH.
+    intros * Hwfgp Hwflp Hpassoc Hfairl.
+    pfold.
+    pinversion Hpassoc;try apply path_assoc_mon;subst.
+    {
+        constructor. red;split; intros; simpl in H; easy.
+    }
+    constructor.
+    { 
+        red;split; intros;
+        pinversion Hfairl;subst;try apply always_mon;
+        red in H4;
+        simpl in H1;
+
+        [eapply local_send_enabled_global_send_enabled in H1 as Hlc 
+        | eapply local_recv_enabled_global_recv_enabled in H1 as Hlc];
+        try exact Hassoc;try easy;
+        try solve [
+        apply wfg_global_path_head in Hwfgp;easy | apply wf_local_path_head in Hwflp;easy];
+        destruct Hlc as [s' [n' Hr]];
+        
+        specialize (H4 p q s' n'); destruct H4 as [Hlv1 Hlv2];
+        [
+        assert(Hevg: eventually (headComm_global p q) (cocons (g,l) ys)) by (eapply Hlv1;easy)
+        |
+        assert(Hevg: eventually (headComm_global p q) (cocons (g,l) ys)) by (eapply Hlv2;easy)];
+        eapply path_assoc_reflects_liveness_helper with (ys:=(cocons (g,l) ys));try easy;
+        pfold;easy.
+    }
+    {
+        right. eapply CIH with (gp := ys);
+        eapply always_tail in Hwfgp, Hwflp, Hfairl;try easy.
+    }
+Qed.
 
 Definition g_by_gamma_trans : forall t p q ell g t', wfgC g -> tctx_wf t -> assoc t g ->
 tctxR t (lcomm p q ell) t' ->
@@ -622,7 +866,7 @@ Proof.
            destruct l;
         pose proof Hvalid as Hvalid'; pinversion Hvalid'; try apply valid_path_mon;try tauto;subst.
         rewrite (coseq_eq (conj_path _ _ _ _ _ _ _ _   )). simpl.
-        
+
         destruct (g_by_gamma_trans t n n0 n1 g x Hwfg Htxwf Hassoc) (eqn:Hyg).
         Check eq_rec_r.
 
